A ton of work on CBPV

CBPV/Normal.lean
@@ -2,15 +2,13 @@ import CBPV.Syntax
 
 open ValType ComType Val Com
 
+def SNeVal (v : Val) : Prop := ∃ x, v = var x
+def SNeVal.var {x} : SNeVal (var x) := ⟨_, rfl⟩
+
 section
 set_option hygiene false
-local infix:40 "⤳" => SRVal
-local infix:40 "⤳" => SRCom
-
+local infix:40 "⤳" => SR
 mutual
-inductive SNeVal : Val → Prop where
-  | var {x} : SNeVal (var x)
-
 inductive SNeCom : Com → Prop where
   | force {v} : SNeVal v → SNeCom (force v)
   | app {m v} : SNeCom m → SNVal v → SNeCom (app m v)
@@ -18,12 +16,11 @@ inductive SNeCom : Com → Prop where
   | case {v m n} : SNeVal v → SNCom m → SNCom n → SNeCom (case v m n)
 
 inductive SNVal : Val → Prop where
+  | var {x} : SNVal (var x)
   | unit : SNVal unit
   | inl {v} : SNVal v → SNVal (inl v)
   | inr {v} : SNVal v → SNVal (inr v)
   | thunk {m} : SNCom m → SNVal (thunk m)
-  | ne {v} : SNeVal v → SNVal v
-  | red {v w : Val} : v ⤳ w → SNVal w → SNVal v
 
 inductive SNCom : Com → Prop where
   | lam {m} : SNCom m → SNCom (lam m)
@@ -31,37 +28,57 @@ inductive SNCom : Com → Prop where
   | ne {m} : SNeCom m → SNCom m
   | red {m n : Com} : m ⤳ n → SNCom n → SNCom m
 
-inductive SRVal : Val → Val → Prop where
-  | inl {v w : Val} : v ⤳ w → inl v ⤳ inl w
-  | inr {v w : Val} : v ⤳ w → inr v ⤳ inr w
-  | thunk {m n : Com} : m ⤳ n → thunk m ⤳ thunk n
-
-inductive SRCom : Com → Com → Prop where
+inductive SR : Com → Com → Prop where
   | thunk {m} : force (thunk m) ⤳ m
   | lam {m : Com} {v} : SNVal v → app (lam m) v ⤳ m⦃v⦄
   | ret {v m} : SNVal v → letin (ret v) m ⤳ m⦃v⦄
-  | inl {v m n} : SNCom n → case (inl v) m n ⤳ m⦃v⦄
-  | inr {v m n} : SNCom m → case (inr v) m n ⤳ n⦃v⦄
-  | force {v w : Val} : v ⤳ w → force v ⤳ force w
-  | app {m n : Com} {v} : m ⤳ n → app m v ⤳ app n v
-  | letin {m m' n : Com} : m ⤳ m' → letin m n ⤳ letin m' n
-  | case {v w : Val} {m n} : v ⤳ w → case v m n ⤳ case w m n
+  | inl {v m n} : SNVal v → SNCom m → SNCom n → case (inl v) m n ⤳ m⦃v⦄
+  | inr {v m n} : SNVal v → SNCom m → SNCom n → case (inr v) m n ⤳ n⦃v⦄
+  | app {m n : Com} {v} : SNVal v → m ⤳ n → app m v ⤳ app n v
+  | letin {m m' n : Com} : SNCom n → m ⤳ m' → letin m n ⤳ letin m' n
 end
 end
+infix:40 "⤳" => SR
 
-infix:40 "⤳" => SRVal
-infix:40 "⤳" => SRCom
+/-*-----------------------------------------
+  Inversion lemmas on strong normalization
+-----------------------------------------*-/
 
--- Inversion on strong normalization of `force`
-theorem SNCom.force_inv {v : Val} (h : SNCom (force v)) : SNVal v := by
+theorem SNCom.force_inv {v} (h : SNCom (force v)) : SNVal v := by
   generalize e : force v = m at h
   mutual_induction h generalizing v
   all_goals first | contradiction | subst e
-  case ne sne => cases sne with | _ snev => exact .ne snev
+  case ne sne => match sne with
+  | .force ⟨_, e⟩ => subst e; exact .var
+  case red sn ih r => cases r; exact .thunk sn
+
+theorem SNCom.case_inv {v m₁ m₂} (h : SNCom (case v m₁ m₂)) : SNVal v ∧ SNCom m₁ ∧ SNCom m₂ := by
+  generalize e : case v m₁ m₂ = n at h
+  mutual_induction h generalizing v m₁ m₂
+  all_goals first | contradiction | subst e
+  case ne sne =>
+    match sne with
+    | .case ⟨_, e⟩ snm₁ snm₂ => subst e; exact ⟨.var, snm₁, snm₂⟩
   case red sn ih r =>
     cases r
-    case thunk => exact .thunk sn
-    case force r => exact .red r (ih rfl)
+    case inl snv snm₁ snm₂ => exact ⟨.inl snv, snm₁, snm₂⟩
+    case inr snv snm₁ snm₂ => exact ⟨.inr snv, snm₁, snm₂⟩
+
+theorem SNCom.lam_inv {m} (h : SNCom (.lam m)) : SNCom m := by
+  generalize e : Com.lam m = n at h
+  mutual_induction h generalizing m
+  all_goals first | contradiction | injection e | subst e
+  case lam e => subst e; assumption
+  case ne sne => cases sne
+  case red r => cases r
+
+theorem SNCom.ret_inv {v} (h : SNCom (.ret v)) : SNVal v := by
+  generalize e : Com.ret v = m at h
+  mutual_induction h generalizing v
+  all_goals first | contradiction | injection e | subst e
+  case ret e => subst e; assumption
+  case ne sne => cases sne
+  case red r => cases r
 
 /-*---------------------------------------
   Transitive closure of strong reduction
@@ -69,72 +86,39 @@ theorem SNCom.force_inv {v : Val} (h : SNCom (force v)) : SNVal v := by
 
 section
 set_option hygiene false
-local infix:40 "⤳⋆" => SRVals
-inductive SRVals : Val → Val → Prop where
-  | refl {v : Val} : v ⤳⋆ v
-  | trans {u v w : Val} : u ⤳ v → v ⤳⋆ w → u ⤳⋆ w
-
-local infix:40 "⤳⋆" => SRComs
-inductive SRComs : Com → Com → Prop where
+local infix:40 "⤳⋆" => SRs
+inductive SRs : Com → Com → Prop where
   | refl {m : Com} : m ⤳⋆ m
   | trans {k m n : Com} : k ⤳ m → m ⤳⋆ n → k ⤳⋆ n
 end
+infix:40 "⤳⋆" => SRs
 
-infix:40 "⤳⋆" => SRVals
-infix:40 "⤳⋆" => SRComs
+@[refl] def SRs.rfl {m} := @SRs.refl m
 
-@[refl] def SRVals.rfl {v} := @SRVals.refl v
-@[refl] def SRComs.rfl {m} := @SRComs.refl m
+def SRs.once {m n : Com} (r : m ⤳ n) : m ⤳⋆ n := .trans r .refl
 
-def SRVals.once {u v : Val} (r : u ⤳ v) : u ⤳⋆ v := .trans r .refl
-def SRComs.once {m n : Com} (r : m ⤳ n) : m ⤳⋆ n := .trans r .refl
-
-theorem SRVals.trans' {u v w : Val} (r₁ : u ⤳⋆ v) (r₂ : v ⤳⋆ w) : u ⤳⋆ w := by
-  induction r₁ generalizing w
-  case refl => exact r₂
-  case trans r _ ih => exact .trans r (ih r₂)
-
-theorem SRComs.trans' {k m n : Com} (r₁ : k ⤳⋆ m) (r₂ : m ⤳⋆ n) : k ⤳⋆ n := by
+theorem SRs.trans' {k m n : Com} (r₁ : k ⤳⋆ m) (r₂ : m ⤳⋆ n) : k ⤳⋆ n := by
   induction r₁ generalizing n
   case refl => exact r₂
   case trans r _ ih => exact .trans r (ih r₂)
 
-instance : Trans SRVals SRVals SRVals where
-  trans := SRVals.trans'
-
-instance : Trans SRComs SRComs SRComs where
-  trans := SRComs.trans'
+instance : Trans SRs SRs SRs where
+  trans := SRs.trans'
 
 /-*--------------------------------
   Congruence and inversion lemmas
   on strong reduction as needed
 --------------------------------*-/
 
-theorem SRComs.force {v w : Val} (r : v ⤳⋆ w) : force v ⤳⋆ force w := by
+theorem SRs.app {m n : Com} {v} (r : m ⤳⋆ n) (snv : SNVal v): app m v ⤳⋆ app n v := by
   induction r
   case refl => exact .refl
-  case trans r₁ _ r₂ => exact .trans (.force r₁) r₂
+  case trans r₁ _ r₂ => exact .trans (.app snv r₁) r₂
 
-theorem SRComs.app {m n : Com} {v} (r : m ⤳⋆ n) : app m v ⤳⋆ app n v := by
+theorem SRs.letin {m m' n : Com} (r : m ⤳⋆ m') (snn : SNCom n) : letin m n ⤳⋆ letin m' n := by
   induction r
   case refl => exact .refl
-  case trans r₁ _ r₂ => exact .trans (.app r₁) r₂
-
-theorem SRComs.letin {m m' n : Com} (r : m ⤳⋆ m') : letin m n ⤳⋆ letin m' n := by
-  induction r
-  case refl => exact .refl
-  case trans r₁ _ r₂ => exact .trans (.letin r₁) r₂
-
-theorem SRComs.case {v w : Val} {m n} (r : v ⤳⋆ w) : case v m n ⤳⋆ case w m n := by
-  induction r
-  case refl => exact .refl
-  case trans r₁ _ r₂ => exact .trans (.case r₁) r₂
-
-theorem SRVals.unit_inv {v : Val} (r : v ⤳⋆ .unit) : v = .unit := by
-  generalize e : Val.unit = w at r
-  induction r
-  case refl => rfl
-  case trans r _ ih => rw [ih e] at r; subst e; cases r
+  case trans r₁ _ r₂ => exact .trans (.letin snn r₁) r₂
 
 /-*----------------------------------------
   Backward closure wrt strong reduction
@@ -142,19 +126,7 @@ theorem SRVals.unit_inv {v : Val} (r : v ⤳⋆ .unit) : v = .unit := by
   e.g. force (thunk (force x)) ⤳ force x
 ----------------------------------------*-/
 
-theorem SRComs.closure {m n : Com} (r : m ⤳⋆ n) (h : SNCom n) : SNCom m := by
-  induction r
-  case refl => assumption
-  case trans r _ ih => exact .red r (ih h)
-
-theorem SRVals.closure {v w : Val} (r : v ⤳⋆ w) (h : SNeVal w) : SNeVal v := by
-  cases h
-  generalize e : Val.var _ = w at r
-  induction r
-  case refl => subst e; constructor
-  case trans r _ ih => cases ih e; cases r
-
-theorem SRVals.closure' {v w : Val} (r : v ⤳⋆ w) (h : SNVal w) : SNVal v := by
+theorem SRs.closure {m n : Com} (r : m ⤳⋆ n) (h : SNCom n) : SNCom m := by
   induction r
   case refl => assumption
   case trans r _ ih => exact .red r (ih h)
@@ -164,27 +136,23 @@ theorem SRVals.closure' {v w : Val} (r : v ⤳⋆ w) (h : SNVal w) : SNVal v := 
 --------------------------------*-/
 
 theorem antirenaming {ξ} :
-  (∀ {v}, SNeVal (renameVal ξ v) → SNeVal v) ∧
   (∀ {m}, SNeCom (renameCom ξ m) → SNeCom m) ∧
   (∀ {v}, SNVal  (renameVal ξ v) → SNVal v)  ∧
   (∀ {m}, SNCom  (renameCom ξ m) → SNCom m)  ∧
-  (∀ {v w}, SRVal (renameVal ξ v) w → ∃ w', w = renameVal ξ w' ∧ SRVal v w') ∧
-  (∀ {m n}, SRCom (renameCom ξ m) n → ∃ n', n = renameCom ξ n' ∧ SRCom m n') := by
-  refine ⟨λ snev ↦ ?sneval, λ snem ↦ ?snecom,
-          λ snv  ↦ ?snval,  λ snm  ↦ ?sncom,
-          λ r    ↦ ?srval,  λ r    ↦ ?srcom⟩
+  (∀ {m n}, renameCom ξ m ⤳ n → ∃ n', n = renameCom ξ n' ∧ m ⤳ n') := by
+  refine ⟨λ snem ↦ ?snecom, λ snv ↦ ?snval, λ snm ↦ ?sncom, λ r ↦ ?srcom⟩
   case' srcom  => generalize e : renameCom ξ _ = m' at r
-  case' srval  => generalize e : renameVal ξ _ = v' at r
   case' sncom  => generalize e : renameCom ξ _ = m' at snm
   case' snval  => generalize e : renameVal ξ _ = v' at snv
   case' snecom => generalize e : renameCom ξ _ = m' at snem
-  case' sneval => generalize e : renameVal ξ _ = v' at snev
-  mutual_induction snev, snem, snv, snm, r, r generalizing ξ
-  case sneval.var v => cases v <;> injection e; constructor
+  mutual_induction snem, snv, snm, r generalizing ξ
   case snecom.force ih m =>
     cases m <;> try contradiction
     injection e with e
-    exact .force (ih e)
+    case force v =>
+    let ⟨_, e⟩ := ih; subst e
+    cases v <;> try contradiction
+    exact .force .var
   case snecom.app ihm ihv m =>
     cases m <;> try contradiction
     injection e with em ev
@@ -193,10 +161,16 @@ theorem antirenaming {ξ} :
     cases m <;> try contradiction
     injection e with em en
     exact .letin (ihm em) (ihn en)
-  case snecom.case ihv ihm ihn m =>
+  case snecom.case snev _ ihv ihm ihn m =>
     cases m <;> try contradiction
     injection e with ev em en
-    refine .case (ihv ev) (ihm em) (ihn en)
+    case case v _ _ =>
+    let ⟨_, e⟩ := snev; subst e
+    cases v <;> try contradiction
+    refine .case .var (ihm em) (ihn en)
+  case snval.var ih v =>
+    cases v <;> try contradiction
+    exact .var
   case snval.unit v => cases v <;> injection e; constructor
   case snval.inl ih v =>
     cases v <;> try contradiction
@@ -210,10 +184,6 @@ theorem antirenaming {ξ} :
     cases v <;> try contradiction
     injection e with e
     exact .thunk (ih e)
-  case snval.ne ih _ => exact .ne (ih e)
-  case snval.red ihr ihv _ =>
-    let ⟨_, e, r⟩ := ihr e
-    exact .red r (ihv (Eq.symm e))
   case sncom.lam ih m =>
     cases m <;> try contradiction
     injection e with e
@@ -226,22 +196,7 @@ theorem antirenaming {ξ} :
   case sncom.red ihr ihm _ =>
     let ⟨_, e, r⟩ := ihr e
     exact .red r (ihm (Eq.symm e))
-  case srval.inl ih v =>
-    cases v <;> try contradiction
-    injection e with e
-    let ⟨_, e, r⟩ := ih e; subst e
-    exact ⟨.inl _, rfl, .inl r⟩
-  case srval.inr ih v =>
-    cases v <;> try contradiction
-    injection e with e
-    let ⟨_, e, r⟩ := ih e; subst e
-    exact ⟨.inr _, rfl, .inr r⟩
-  case srval.thunk ih v =>
-    cases v <;> try contradiction
-    injection e with e
-    let ⟨_, e, r⟩ := ih e; subst e
-    exact ⟨.thunk _, rfl, .thunk r⟩
-  case srcom.thunk m =>
+  case srcom.thunk ih m =>
     cases m <;> try contradiction
     injection e with e
     case force v =>
@@ -264,53 +219,43 @@ theorem antirenaming {ξ} :
     injection ev with ev
     subst ev em; rw [renameDist]
     exact ⟨_, rfl, .ret (ih rfl)⟩
-  case srcom.inl ih m =>
+  case srcom.inl ihv ihm ihn m =>
     cases m <;> try contradiction
     injection e with ev em en
     rename Val => v
     cases v <;> try contradiction
     injection ev with ev
-    subst ev em; rw [renameDist]
-    exact ⟨_, rfl, .inl (ih en)⟩
-  case srcom.inr ih m =>
+    subst ev em en; rw [renameDist]
+    exact ⟨_, rfl, .inl (ihv rfl) (ihm rfl) (ihn rfl)⟩
+  case srcom.inr ihv ihm ihn m =>
     cases m <;> try contradiction
     injection e with ev em en
     rename Val => v
     cases v <;> try contradiction
     injection ev with ev
-    subst ev en; rw [renameDist]
-    exact ⟨_, rfl, .inr (ih em)⟩
-  case srcom.force ih m =>
-    cases m <;> try contradiction
-    injection e with e
-    let ⟨_, e, r⟩ := ih e; subst e
-    exact ⟨.force _, rfl, .force r⟩
-  case srcom.app ih m =>
+    subst ev em en; rw [renameDist]
+    exact ⟨_, rfl, .inr (ihv rfl) (ihm rfl) (ihn rfl)⟩
+  case srcom.app ihv ihm m =>
     cases m <;> try contradiction
     injection e with em ev
-    let ⟨_, em, r⟩ := ih em; subst em ev
-    exact ⟨.app _ _, rfl, .app r⟩
-  case srcom.letin ih m =>
+    let ⟨_, em, r⟩ := ihm em; subst em ev
+    exact ⟨.app _ _, rfl, .app (ihv rfl) r⟩
+  case srcom.letin ihn ihm  m =>
     cases m <;> try contradiction
     injection e with em ev
-    let ⟨_, em, r⟩ := ih em; subst em ev
-    exact ⟨.letin _ _, rfl, .letin r⟩
-  case srcom.case ih m =>
-    cases m <;> try contradiction
-    injection e with ev em en
-    let ⟨w, ev, r⟩ := ih ev; subst ev em en
-    exact ⟨.case _ _ _, rfl, .case r⟩
+    let ⟨_, em, r⟩ := ihm em; subst em ev
+    exact ⟨.letin _ _, rfl, .letin (ihn rfl) r⟩
 
-def SNCom.antirenaming {ξ m} := @(@_root_.antirenaming ξ).right.right.right.left m
+def SNCom.antirenaming {ξ m} := @(@_root_.antirenaming ξ).right.right.left m
 
 theorem extensionality {m x} (h : SNCom (app m (var x))) : SNCom m := by
   generalize e : app m (var x) = m' at h
   mutual_induction h generalizing m x
   all_goals first | contradiction | subst e
-  case ne h => cases h with | _ snem => exact .ne snem
+  case ne h => cases h with | app snem => exact .ne snem
   case red r =>
     cases r
     case lam snm _ =>
       rw [substToRename] at snm
       exact .lam (SNCom.antirenaming snm)
-    case app r _ h => exact .red r (h rfl)
+    case app r _ _ h => exact .red r (h rfl)
