CBPV/Reduction.lean
@@ -1,0 +1,426 @@
+import CBPV.Normal
+
+open Val Com
+
+/-*----------------------
+  Single-step reduction
+----------------------*-/
+
+section
+set_option hygiene false
+local infix:40 "⤳ᵛ" => StepVal
+local infix:40 "⤳ᶜ" => StepCom
+
+mutual
+inductive StepVal : Val → Val → Prop where
+  | inl {v w} : v ⤳ᵛ w → inl v ⤳ᵛ inl w
+  | inr {v w} : v ⤳ᵛ w → inr v ⤳ᵛ inr w
+  | thunk {m n} : m ⤳ᶜ n → thunk m ⤳ᵛ thunk n
+
+inductive StepCom : Com → Com → Prop where
+  | π {m} : force (thunk m) ⤳ᶜ m
+  | β {m v} : app (lam m) v ⤳ᶜ m⦃v⦄
+  | ζ {v m} : letin (ret v) m ⤳ᶜ m⦃v⦄
+  | ιl {v m n} : case (inl v) m n ⤳ᶜ m⦃v⦄
+  | ιr {v m n} : case (inr v) m n ⤳ᶜ n⦃v⦄
+  | force {v w} : v ⤳ᵛ w → force v ⤳ᶜ force w
+  | lam {m n} : m ⤳ᶜ n → lam m ⤳ᶜ lam n
+  | app₁ {m n v} :
+    m ⤳ᶜ n →
+    -------------------
+    app m v ⤳ᶜ app n v
+  | app₂ {m v w} :
+    v ⤳ᵛ w →
+    -------------------
+    app m v ⤳ᶜ app m w
+  | ret {v w} : v ⤳ᵛ w → ret v ⤳ᶜ ret w
+  | letin₁ {m m' n} :
+    m ⤳ᶜ m' →
+    ------------------------
+    letin m n ⤳ᶜ letin m' n
+  | letin₂ {m n n'} :
+    n ⤳ᶜ n' →
+    ------------------------
+    letin m n ⤳ᶜ letin m n'
+  | case {v w m n} :
+    v ⤳ᵛ w →
+    -------------------------
+    case v m n ⤳ᶜ case w m n
+  | case₁ {v m m' n} :
+    m ⤳ᶜ m' →
+    --------------------------
+    case v m n ⤳ᶜ case v m' n
+  | case₂ {v m n n'} :
+    n ⤳ᶜ n' →
+    --------------------------
+    case v m n ⤳ᶜ case v m n'
+end
+end
+
+infix:40 "⤳ᵛ" => StepVal
+infix:40 "⤳ᶜ" => StepCom
+
+/-*---------------------
+  Multi-step reduction
+---------------------*-/
+
+section
+set_option hygiene false
+local infix:40 "⤳⋆ᵛ" => StepVals
+local infix:40 "⤳⋆ᶜ" => StepComs
+
+inductive StepVals : Val → Val → Prop where
+  | refl {a} : a ⤳⋆ᵛ a
+  | trans {a b c} : a ⤳ᵛ b → b ⤳⋆ᵛ c → a ⤳⋆ᵛ c
+
+inductive StepComs : Com → Com → Prop where
+  | refl {a} : a ⤳⋆ᶜ a
+  | trans {a b c} : a ⤳ᶜ b → b ⤳⋆ᶜ c → a ⤳⋆ᶜ c
+end
+
+infix:40 "⤳⋆ᵛ" => StepVals
+infix:40 "⤳⋆ᶜ" => StepComs
+
+def StepVals.once {a b} (r : a ⤳ᵛ b) : a ⤳⋆ᵛ b := .trans r .refl
+def StepComs.once {a b} (r : a ⤳ᶜ b) : a ⤳⋆ᶜ b := .trans r .refl
+
+theorem StepVals.trans' {a b c} (r₁ : a ⤳⋆ᵛ b) (r₂ : b ⤳⋆ᵛ c) : a ⤳⋆ᵛ c := by
+  induction r₁ generalizing c
+  case refl => exact r₂
+  case trans r₁ _ ih => exact .trans r₁ (ih r₂)
+
+theorem StepComs.trans' {a b c} (r₁ : a ⤳⋆ᶜ b) (r₂ : b ⤳⋆ᶜ c) : a ⤳⋆ᶜ c := by
+  induction r₁ generalizing c
+  case refl => exact r₂
+  case trans r₁ _ ih => exact .trans r₁ (ih r₂)
+
+/-*-----------------------------------------
+  Congruence rules on multi-step reduction
+-----------------------------------------*-/
+
+theorem StepComs.app₁ {m n v} (r : m ⤳⋆ᶜ n) : app m v ⤳⋆ᶜ app n v := by
+  induction r
+  case refl => exact .refl
+  case trans r₁ _ r₂ => exact .trans (.app₁ r₁) r₂
+
+theorem StepComs.app₂ {m v w} (r : v ⤳⋆ᵛ w) : app m v ⤳⋆ᶜ app m w := by
+  induction r
+  case refl => exact .refl
+  case trans r₁ _ r₂ => exact .trans (.app₂ r₁) r₂
+
+/-*---------------------------------
+  Traditional strong normalization
+---------------------------------*-/
+
+inductive StepVal.SN : Val → Prop where
+  | sn {v} : (∀ {w}, v ⤳ᵛ w → StepVal.SN w) → StepVal.SN v
+
+inductive StepCom.SN : Com → Prop where
+  | sn {m} : (∀ {n}, m ⤳ᶜ n → StepCom.SN n) → StepCom.SN m
+
+theorem StepVals.SN {v w} (r : v ⤳⋆ᵛ w) (h : StepVal.SN v) : StepVal.SN w := by
+  induction r
+  case refl => assumption
+  case trans r _ ih => cases h with | _ ihSN => exact ih (ihSN r)
+
+theorem StepComs.SN {m n} (r : m ⤳⋆ᶜ n) (h : StepCom.SN m) : StepCom.SN n := by
+  induction r
+  case refl => assumption
+  case trans r _ ih => cases h with | _ ihSN => exact ih (ihSN r)
+
+/-*-----------------------
+  Inversion lemmas on SN
+-----------------------*-/
+
+theorem StepVal.SN.inl_inv {v} (h : StepVal.SN (.inl v)) : StepVal.SN v := by
+  generalize e : Val.inl v = w at h
+  induction h generalizing v; subst e
+  case sn ih =>
+  constructor; intro _ r
+  exact ih (.inl r) rfl
+
+theorem StepVal.SN.thunk_inv {m} (h : StepVal.SN (.thunk m)) : StepCom.SN m := by
+  generalize e : Val.thunk m = v at h
+  induction h generalizing m; subst e
+  case sn ih =>
+  constructor; intro _ r
+  exact ih (.thunk r) rfl
+
+theorem StepCom.SN.lam_inv {m} (h : StepCom.SN (.lam m)) : StepCom.SN m := by
+  generalize e : Com.lam m = n at h
+  induction h generalizing m; subst e
+  case sn ih =>
+  constructor; intro _ r
+  exact ih (.lam r) rfl
+
+theorem StepCom.SN.app_inv {m v} (h : StepCom.SN (.app m v)) : StepCom.SN m := by
+  generalize e : Com.app m v = n at h
+  induction h generalizing m; subst e
+  case sn ih =>
+  constructor; intro _ r
+  exact ih (.app₁ r) rfl
+
+theorem StepCom.SN.letin_inv {m₁ m₂} (h : StepCom.SN (.letin m₁ m₂)) : StepCom.SN m₁ := by
+  generalize e : Com.letin m₁ m₂ = n at h
+  induction h generalizing m₁; subst e
+  case sn ih =>
+  constructor; intro _ r
+  exact ih (.letin₁ r) rfl
+
+/-*-----------------------
+  Congruence rules on SN
+-----------------------*-/
+
+theorem StepVal.SN.inl {v} (h : StepVal.SN v) : StepVal.SN (.inl v) := by
+  induction h; constructor; intro _ r; cases r
+  case _ ih _ r => exact ih r
+
+theorem StepVal.SN.inr {v} (h : StepVal.SN v) : StepVal.SN (.inr v) := by
+  induction h; constructor; intro _ r; cases r
+  case _ ih _ r => exact ih r
+
+theorem StepVal.SN.thunk {m} (h : StepCom.SN m) : StepVal.SN (.thunk m) := by
+  induction h; constructor; intro _ r; cases r
+  case _ ih _ r => exact ih r
+
+theorem StepCom.SN.force {v} (h : StepVal.SN v) : StepCom.SN (.force v) := by
+  induction h; constructor; intro _ r; cases r
+  case π h _ => exact (StepVal.SN.sn h).thunk_inv
+  case force ih _ r => exact ih r
+
+theorem StepCom.SN.lam {m} (h : StepCom.SN m) : StepCom.SN (.lam m) := by
+  induction h; constructor; intro _ r; cases r
+  case _ ih _ r => exact ih r
+
+theorem StepCom.SN.ret {v} (h : StepVal.SN v) : StepCom.SN (.ret v) := by
+  induction h; constructor; intro _ r; cases r
+  case _ ih _ r => exact ih r
+
+/-*--------------
+  SN on redexes
+--------------*-/
+
+theorem StepCom.SN.force_thunk {m} (snm : StepCom.SN m) : StepCom.SN (.force (.thunk m)) := by
+  induction snm
+  constructor; intro _ r; cases r
+  case a.π h _ => exact .sn h
+  case a.force ih _ r =>
+    cases r with | thunk r => exact ih r
+
+theorem StepCom.SN.app_lam {m v} (snv : StepVal.SN v) (snm : StepCom.SN (m⦃v⦄)) : StepCom.SN (Com.app (Com.lam m) v) := by
+  generalize e : (m⦃v⦄) = n at snm
+  induction snm generalizing m v; subst e
+  constructor; intro _ r; cases r
+  case a.β h _ => exact .sn h
+  case a.app₁ ih _ r =>
+    cases r with | lam r =>
+    refine ih ?_ snv rfl; sorry -- substitution
+  case a.app₂ ih _ r =>
+    cases snv with | sn h =>
+    refine ih ?_ (h r) rfl; sorry -- substitution
+
+theorem StepCom.SN.letin_ret {m v} (snv : StepVal.SN v) (snm : StepCom.SN (m⦃v⦄)) : StepCom.SN (Com.letin (Com.ret v) m) := by
+  generalize e : (m⦃v⦄) = n at snm
+  induction snm generalizing m v; subst e
+  constructor; intro _ r; cases r
+  case a.ζ h _ => exact .sn h
+  case a.letin₁ ih _ r =>
+    cases r with | ret r =>
+    cases snv with | sn h =>
+    refine ih ?_ (h r) rfl; sorry -- substitution
+  case a.letin₂ ih _ r =>
+    refine ih ?_ snv rfl; sorry -- substitution
+
+theorem StepCom.SN.case_inl {v m n} (snv : StepVal.SN v) (snm : StepCom.SN (m⦃v⦄)) (snn : StepCom.SN n) : StepCom.SN (.case (.inl v) m n) := by
+  generalize e : (m⦃v⦄) = m' at snm
+  induction snm generalizing v m n; subst e
+  constructor; intro _ r; cases r
+  case a.ιl h _ => exact .sn h
+  case a.case ih _ r =>
+    cases r with | inl r =>
+    cases snv with | sn h =>
+    refine ih ?_ (h r) snn rfl; sorry -- substitution
+  case a.case₁ ih _ r =>
+    refine ih ?_ snv snn rfl; sorry -- substitution
+  case a.case₂ ih _ r =>
+    cases snn with | sn h =>
+    refine ih ?_ snv (h r) rfl; sorry -- substitution
+
+theorem StepCom.SN.case_inr {v m n} (snv : StepVal.SN v) (snm : StepCom.SN m) (snn : StepCom.SN (n⦃v⦄)) : StepCom.SN (.case (.inr v) m n) := by
+  generalize e : (n⦃v⦄) = n' at snn
+  induction snn generalizing v m n; subst e
+  constructor; intro _ r; cases r
+  case a.ιr h _ => exact .sn h
+  case a.case ih _ r =>
+    cases r with | inr r =>
+    cases snv with | sn h =>
+    refine ih ?_ (h r) snm rfl; sorry -- substitution
+  case a.case₁ ih _ r =>
+    cases snm with | sn h =>
+    refine ih ?_ snv (h r) rfl; sorry -- substitution
+  case a.case₂ ih _ r =>
+    refine ih ?_ snv snm rfl; sorry -- substitution
+
+/-*------------------------
+  Backward closure of SN
+  (depends on confluence)
+------------------------*-/
+
+section
+set_option hygiene false
+local infix:40 "⤳ⁿ" => StepSN
+inductive StepSN : Com → Com → Prop where
+  | thunk {m} : force (thunk m) ⤳ⁿ m
+  | lam {m : Com} {v} : StepVal.SN v → app (lam m) v ⤳ⁿ m⦃v⦄
+  | ret {v m} : StepVal.SN v → letin (ret v) m ⤳ⁿ m⦃v⦄
+  | inl {v m n} : StepVal.SN v → StepCom.SN m → StepCom.SN n → case (inl v) m n ⤳ⁿ m⦃v⦄
+  | inr {v m n} : StepVal.SN v → StepCom.SN m → StepCom.SN n → case (inr v) m n ⤳ⁿ n⦃v⦄
+  | app {m n : Com} {v} : StepVal.SN v → m ⤳ⁿ n → app m v ⤳ⁿ app n v
+  | letin {m m' n : Com} : StepCom.SN n → m ⤳ⁿ m' → letin m n ⤳ⁿ letin m' n
+end
+infix:40 "⤳ⁿ" => StepSN
+
+theorem confluence {m n₁ n₂} (r₁ : m ⤳ᶜ n₁) (r₂ : m ⤳ⁿ n₂) : (∃ m', n₁ ⤳ⁿ m' ∧ n₂ ⤳ᶜ m') ∨ n₁ = n₂ := by
+  induction r₂ generalizing n₁ <;> cases r₁
+  case lam.β => exact .inr rfl
+  case lam.app₁ snv _ r =>
+    cases r; case lam r =>
+    refine .inl ⟨_, .lam snv, ?_⟩; sorry -- substitution
+  case lam.app₂ snv _ r =>
+    cases snv; case sn h =>
+    refine .inl ⟨_, .lam (h r), ?_⟩; sorry -- substitution
+  case app.β r ih => cases r
+  case app.app₁ snv _ ih _ r =>
+    cases ih r
+    case inl h =>
+      let ⟨_, r₁', r₂'⟩ := h
+      refine .inl ⟨_, .app snv r₁', .app₁ r₂'⟩
+    case inr e => subst e; exact .inr rfl
+  case app.app₂ snv r₁' _ _ r₂' =>
+    cases snv; case sn h =>
+    refine .inl ⟨_, .app (h r₂') r₁', .app₂ r₂'⟩
+  all_goals sorry
+
+theorem StepSN.closure {m n} (r : m ⤳ⁿ n) (snn : StepCom.SN n) : StepCom.SN m := by
+  induction r
+  case thunk => exact .force_thunk snn
+  case lam snv => exact .app_lam snv snn
+  case ret snv => exact .letin_ret snv snn
+  case inl snv _ snm => exact .case_inl snv snn snm
+  case inr snv snm _ => exact .case_inr snv snm snn
+  case app rn ih =>
+    let snm := ih snn.app_inv
+    sorry -- property 3.13 (1)
+  case letin rn ih =>
+    let snm := ih snn.letin_inv
+    sorry -- another property
+
+/-*--------------
+  Neutral terms
+--------------*-/
+
+@[simp, reducible] def NeVal (v : Val) : Prop := ∃ x, v = var x
+@[simp, reducible] def NeCom (m : Com) : Prop :=
+  match m with
+  | force v => NeVal v
+  | app m _ => NeCom m
+  | letin m _ => NeCom m
+  | case v _ _ => NeVal v
+  | _ => False
+
+theorem preservation :
+  (∀ {v w}, v ⤳ᵛ w → NeVal v → NeVal w) ∧
+  (∀ {m n}, m ⤳ᶜ n → NeCom m → NeCom n) := by
+  refine ⟨λ r ↦ ?neval, λ r ↦ ?necom⟩
+  mutual_induction r, r
+  all_goals intro ne; try simp at *
+  case necom.force ih | necom.case ih => let ⟨x, e⟩ := ne; exact ih x e
+  all_goals apply_rules
+
+def StepVal.preservation {v w} := @_root_.preservation.left  v w
+def StepCom.preservation {m n} := @_root_.preservation.right m n
+
+/-*----------------------------------
+  Congruence rules on neutral terms
+----------------------------------*-/
+
+theorem StepCom.SN.app {m v} (nem : NeCom m) (snm : StepCom.SN m) (snv : StepVal.SN v) : StepCom.SN (app m v) := by
+  constructor; intro _ r
+  cases r
+  case a.β => cases nem
+  case a.app₁ r =>
+    cases snm
+    case sn h => exact .app (r.preservation nem) (h r) snv
+  case a.app₂ r =>
+    cases snv
+    case sn h => exact .app nem snm (h r)
+termination_by sizeOf snm + sizeOf snv
+decreasing_by all_goals sorry
+
+theorem StepCom.SN.letin {m n} (nem : NeCom m) (snm : StepCom.SN m) (snn : StepCom.SN n) : StepCom.SN (letin m n) := by
+  constructor; intro _ r
+  cases r
+  case a.ζ => cases nem
+  case a.letin₁ r =>
+    cases snm
+    case sn h => exact .letin (r.preservation nem) (h r) snn
+  case a.letin₂ r =>
+    cases snn
+    case sn h => exact .letin nem snm (h r)
+termination_by sizeOf snm + sizeOf snn
+decreasing_by all_goals sorry
+
+theorem StepCom.SN.case {v m n} (nev : NeVal v) (snm : StepCom.SN m) (snn : StepCom.SN n) : StepCom.SN (.case v m n) := by
+  constructor; intro _ r
+  cases r
+  case a.ιl => cases nev; contradiction
+  case a.ιr => cases nev; contradiction
+  case a.case r => cases r <;> cases nev <;> contradiction
+  case a.case₁ r =>
+    cases snm
+    case sn h => exact .case nev (h r) snn
+  case a.case₂ r =>
+    cases snn
+    case sn h => exact .case nev snm (h r)
+termination_by sizeOf snm + sizeOf snn
+decreasing_by all_goals sorry
+
+/-*--------------------------
+  Soundness of SNCom/SNVal
+  wrt StepVal.SN/StepCom.SN
+--------------------------*-/
+
+theorem NeCom.ne {m} (snem : SNeCom m) : NeCom m := by
+  mutual_induction snem <;> assumption
+
+theorem StepVal.SN.ne {v} (h : SNeVal v) : StepVal.SN v := by
+  let ⟨_, e⟩ := h; subst e
+  constructor; intro _ r; cases r
+
+theorem soundness :
+  (∀ {m}, SNeCom m → StepCom.SN m) ∧
+  (∀ {v}, SNVal  v → StepVal.SN v) ∧
+  (∀ {m}, SNCom  m → StepCom.SN m) ∧
+  (∀ {m n : Com}, m ⤳ n → m ⤳ⁿ n) := by
+  refine ⟨λ sne ↦ ?snecom, λ sn ↦ ?snval, λ sn ↦ ?sncom, λ r ↦ ?srcom⟩
+  mutual_induction sne, sn, sn, r
+  case snecom.force ih => exact .force (.ne ih)
+  case snecom.app snem _ snm snv => exact .app (.ne snem) snm snv
+  case snecom.letin snem _ snm snn => exact .letin (.ne snem) snm snn
+  case snecom.case snv _ _ snm snn => exact .case snv snm snn
+  case snval.var => constructor; intro _ r; cases r
+  case snval.unit => constructor; intro _ r; cases r
+  case snval.inl ih => exact .inl ih
+  case snval.inr ih => exact .inr ih
+  case snval.thunk ih => exact .thunk ih
+  case sncom.lam ih => exact .lam ih
+  case sncom.ret ih => exact .ret ih
+  case sncom.ne => assumption
+  case sncom.red r ih => exact r.closure ih
+  case srcom.thunk => constructor
+  case srcom.lam => constructor; assumption
+  case srcom.ret => constructor; assumption
+  case srcom.inl => constructor <;> assumption
+  case srcom.inr => constructor <;> assumption
+  case srcom.app => constructor <;> assumption
+  case srcom.letin => constructor <;> assumption
